PAC_Checker/String_Assn.thy
@@ -1,222 +1,295 @@
 theory String_Assn
-  imports Isabelle_LLVM.LLVM_DS_Open_List Char_Assn
+  imports IICF_Owning_List Char_Assn
 begin
 
-text \<open>Implement Chars as Open Lists\<close>
+text \<open>Implement String by Open List\<close>
 
 type_synonym str = \<open>char list\<close>
 
-term larray_assn
+text \<open>The list interface implementation of \<open>IICF_Open_List\<close> is specialized to
+  strings by instantiating the element assertion with \<open>char_assn\<close>. All interface
+  rules require \<open>is_pure char_assn\<close>, discharged by \<open>char_assn_pure\<close>.\<close>
 
-definition \<open>str_assn \<equiv> hr_comp \<upharpoonleft>os_list_assn (\<langle>the_pure char_assn\<rangle>list_rel)\<close>
-lemma str_assn_pure: \<open>is_pure str_assn\<close>
-  unfolding str_assn_def os_list_assn_def 
-  (* do we have any chance here? I don't think we do... *)
-  oops
+abbreviation strl_assn :: \<open>str \<Rightarrow> 8 word os_list \<Rightarrow> assn\<close> where
+  \<open>strl_assn \<equiv> os_assn char_assn\<close>
 
-(* We have to implement some functions for open lists which are not there yet *)
-definition os_hd :: \<open>'a::llvm_rep os_list \<Rightarrow> 'a llM\<close> where[llvm_code]:
-  \<open>os_hd p = doM { v \<leftarrow> ll_load p; Mreturn (node.val v)}\<close>
+definition \<open>string_rel \<equiv> \<langle>char_rel\<rangle>list_rel\<close>
 
-lemma os_hd_rule[vcg_rules]:
-  \<open>xs \<noteq> [] \<Longrightarrow> llvm_htriple (\<upharpoonleft>os_list_assn xs r) (os_hd r) (\<lambda>x. \<up>(x=hd xs) ** \<upharpoonleft>os_list_assn xs r)\<close>
-  apply (cases xs; simp)
-  unfolding os_hd_def os_list_assn_def
+subsection \<open>Lexicographic Order on Lists\<close>
+
+text \<open>The linear order on lists (lexicographic) is needed already here so that the
+  refinement rule for \<open>strl_lt\<close> can be stated against the abstract \<open>(<)\<close>. It used to live
+  in \<open>PAC_Checker_Relation\<close>, but that theory is downstream of \<open>String_Assn\<close> \<emdash> moving the
+  instantiation up makes \<open>(<) :: str \<Rightarrow> str \<Rightarrow> bool\<close> available here; \<open>PAC_Checker_Relation\<close>
+  inherits it (via \<open>Monom_Assn\<close>).\<close>
+
+instantiation list :: (linorder) linorder
+begin
+  definition less_list where  "less_list = lexordp (<)"
+  definition less_eq_list where "less_eq_list = lexordp_eq"
+
+instance
+proof standard
+  have [dest]: \<open>\<And>x y :: 'a :: linorder list. (x, y) \<in> lexord {(x, y). x < y} \<Longrightarrow>
+           lexordp_eq y x \<Longrightarrow> False\<close>
+    by (metis lexordp_antisym lexordp_conv_lexord lexordp_eq_conv_lexord)
+  have [simp]: \<open>\<And>x y :: 'a :: linorder list. lexordp_eq x y \<Longrightarrow>
+           \<not> lexordp_eq y x \<Longrightarrow>
+           (x, y) \<in> lexord {(x, y). x < y}\<close>
+    using lexordp_conv_lexord lexordp_conv_lexordp_eq by blast
+  show
+   \<open>(x < y) = Restricted_Predicates.strict (\<le>) x y\<close>
+   \<open>x \<le> x\<close>
+   \<open>x \<le> y \<Longrightarrow> y \<le> z \<Longrightarrow> x \<le> z\<close>
+   \<open>x \<le> y \<Longrightarrow> y \<le> x \<Longrightarrow> x = y\<close>
+   \<open>x \<le> y \<or> y \<le> x\<close>
+   for x y z :: \<open>'a :: linorder list\<close>
+    by (auto simp: less_list_def less_eq_list_def List.lexordp_def
+    lexordp_conv_lexord lexordp_into_lexordp_eq lexordp_antisym
+    antisym_def lexordp_eq_refl lexordp_eq_linear intro: lexordp_eq_trans
+    dest: lexordp_eq_antisym)
+qed
+
+end
+
+text \<open>The defining recursion of the list order (matching @{const lexordp}'s \<open>[code]\<close> rules):
+  supplied locally in the order proofs below rather than declared globally \<open>[simp]\<close>, to
+  avoid perturbing downstream simpsets.\<close>
+
+lemma list_less_Nil_left: \<open>(([]::'a::linorder list) < ys) = (ys \<noteq> [])\<close>
+  by (cases ys) (auto simp: less_list_def lexordp_def)
+
+lemma list_less_Nil_right: \<open>(xs < ([]::'a::linorder list)) = False\<close>
+  by (auto simp: less_list_def lexordp_def)
+
+lemma list_less_Cons: \<open>((x # xs) < (y # ys)) = (x < y \<or> (x = y \<and> xs < ys))\<close>
+  for x :: \<open>'a::linorder\<close>
+  by (auto simp: less_list_def lexordp_def)
+
+subsection \<open>String Equality\<close>
+
+text \<open>Instantiation ladder for the generic \<open>os_eq\<close> template: the element comparison for
+  chars is plain \<open>ll_icmp_eq\<close>, correct because \<open>char_rel\<close> is bi-unique (injectivity of
+  \<open>char_of_word\<close>). Feeding the resulting \<open>str_eq_rule\<close> back into \<open>ol_eq_rule\<close> one level
+  up gives monomial equality (\<open>os_eq str_eq\<close> at \<open>ol_assn strl_assn\<close>) \<emdash> no purity needed
+  at that level.\<close>
+
+lemma char_of_word_inj: \<open>char_of_word a = char_of_word b \<longleftrightarrow> a = b\<close>
+proof
+  assume \<open>char_of_word a = char_of_word b\<close>
+  hence \<open>(of_char (char_of_word a) :: nat) = of_char (char_of_word b)\<close> by simp
+  hence \<open>unat a = unat b\<close>
+    unfolding char_of_word_def by (simp add: of_char_of unat_of_char_mod)
+  thus \<open>a = b\<close> by (simp add: word_unat_eq_iff)
+qed simp
+
+text \<open>The element-equality rule in the htriple format expected by \<open>ol_eq_rule\<close>'s premise.
+  Proven in a throwaway \<open>llvm_prim_arith_setup\<close> context (cf. CLAUDE.md); NOT declared
+  \<open>[vcg_rules]\<close> globally \<emdash> a raw \<open>ll_icmp_eq\<close> rule could hijack snat/unat comparisons
+  elsewhere.\<close>
+
+context begin
+interpretation llvm_prim_arith_setup .
+
+lemma char_eq_rule:
+  \<open>llvm_htriple (char_assn a c ** char_assn a' c') (ll_icmp_eq c c')
+    (\<lambda>r. char_assn a c ** char_assn a' c' ** \<upharpoonleft>bool.assn (a = a') r)\<close>
+  unfolding char_assn_def char_rel_def
+  supply [simp] = pure_def in_br_conv bool.assn_def char_of_word_inj
   by vcg
 
-definition os_tl :: \<open>'a::llvm_rep os_list \<Rightarrow> 'a os_list llM\<close> where[llvm_code]:
-  \<open>os_tl p = doM {
-    n \<leftarrow> ll_load p;
-    ll_free p;
-    Mreturn (node.next n)
-  }\<close>
+end
 
-lemma op_tl_rule[vcg_rules]:
-  \<open>xs \<noteq> [] \<Longrightarrow> llvm_htriple (\<upharpoonleft>os_list_assn xs r) (os_tl r) (\<lambda>x. \<upharpoonleft>os_list_assn (tl xs) x)\<close>
-  apply (cases xs; simp)
-  unfolding os_tl_def os_list_assn_def
-  by vcg
+text \<open>First-order specialization of the higher-order template, for code export.\<close>
 
-definition os_list_get :: \<open>'a::llvm_rep os_list \<Rightarrow> 'b::len2 word \<Rightarrow> 'a llM\<close> where [llvm_code]:
-  \<open>os_list_get p\<^sub>0 i\<^sub>0 = doM {
-    (p, _) \<leftarrow> llc_while
-      (\<lambda>(_, i). ll_cmp (i \<noteq> 0))
-      (\<lambda>(p, i). doM {
-        n \<leftarrow> ll_load p; 
-        Mreturn (node.next n, i - 1)
-      }) (p\<^sub>0, i\<^sub>0);
-    n \<leftarrow> ll_load p;
-    Mreturn (node.val n)
-  }\<close>
+definition str_eq :: \<open>8 word os_list \<Rightarrow> 8 word os_list \<Rightarrow> 1 word llM\<close> where
+  \<open>str_eq \<equiv> os_eq ll_icmp_eq\<close>
 
-lemma os_list_get_rule[vcg_rules]:
-  \<open>llvm_htriple
-    (\<upharpoonleft>os_list_assn xs p ** \<upharpoonleft>snat.assn n nn ** \<up>(n < length xs))
-    (os_list_get p nn)
-    (\<lambda>v. \<up>(v = xs ! n) ** \<upharpoonleft>os_list_assn xs p)\<close>
-  unfolding os_list_get_def
-  apply (rewrite annotate_llc_while [where
-    I="\<lambda>(q, ii) t. EXS i. \<upharpoonleft>snat.assn i ii
-                 ** lseg (take i xs) p q
-                 ** lseg (drop i xs) q null
-                 ** \<up>(i \<le> n \<and> 0 \<le> i)
-                 ** \<up>\<^sub>!(t = i)"
-    and R="measure id"])
-  supply [simp] = os_list_assn_def
+lemma str_eq_simps[llvm_code]:
+  \<open>str_eq p q = (
+    if p = null then Mreturn (from_bool (q = null))
+    else if q = null then Mreturn 0
+    else doM {
+      np \<leftarrow> ll_load p; nq \<leftarrow> ll_load q;
+      b \<leftarrow> ll_icmp_eq (node.val np) (node.val nq);
+      if to_bool b then str_eq (node.next np) (node.next nq)
+      else Mreturn 0 })\<close>
+  unfolding str_eq_def by (rule os_eq.simps)
+
+lemma str_eq_rule[vcg_rules]:
+  \<open>llvm_htriple (strl_assn xs p ** strl_assn ys q) (str_eq p q)
+    (\<lambda>r. strl_assn xs p ** strl_assn ys q ** \<upharpoonleft>bool.assn (xs = ys) r)\<close>
+  unfolding str_eq_def
+  by (rule os_eq_rule[where A=char_assn and eqi=ll_icmp_eq, OF char_assn_pure char_eq_rule])
+
+sepref_register \<open>(=) :: char list \<Rightarrow> char list \<Rightarrow> bool\<close>
+
+lemma str_eq_hnr[sepref_fr_rules]:
+  \<open>(uncurry str_eq, uncurry (RETURN oo (=))) \<in> strl_assn\<^sup>k *\<^sub>a strl_assn\<^sup>k \<rightarrow>\<^sub>a bool1_assn\<close>
+  unfolding str_eq_def
+  using ol_eq_hnr[where A=char_assn and eqi=ll_icmp_eq, OF char_eq_rule]
+  unfolding ol_assn_pure_conv[OF char_assn_pure] .
+
+subsection \<open>Lexicographic Order for Strings\<close>
+
+text \<open>Generic template deciding the lexicographic order \<open>xs < ys\<close> on open lists, given an
+  element \<^emph>\<open>strict less\<close> \<open>lti\<close> and an element \<^emph>\<open>equality\<close> \<open>eqi\<close>. The three-way node step
+  mirrors @{const lexordp}'s \<open>[code]\<close> recursion \<open>x < y \<or> (x = y \<and> xs < ys)\<close>: if the heads
+  are strictly ordered we are done (\<open>1\<close>/\<open>0\<close>), if they are equal we recurse, otherwise the
+  left head is the greater one (\<open>0\<close>). The order-agnostic \<^emph>\<open>true\<close>/\<^emph>\<open>false\<close> literals \<open>1\<close>/\<open>0\<close>
+  are \<open>from_bool True\<close>/\<open>from_bool False\<close>. Analogous to @{const os_eq}; not \<open>[llvm_code]\<close>
+  (higher-order in \<open>lti\<close>/\<open>eqi\<close>), so instances are specialized first-order for export.\<close>
+
+partial_function (M) os_less ::
+  \<open>('c::llvm_rep \<Rightarrow> 'c \<Rightarrow> 1 word llM) \<Rightarrow> ('c \<Rightarrow> 'c \<Rightarrow> 1 word llM)
+     \<Rightarrow> 'c os_list \<Rightarrow> 'c os_list \<Rightarrow> 1 word llM\<close> where
+  \<open>os_less lti eqi p q = (
+    if q = null then Mreturn 0
+    else if p = null then Mreturn 1
+    else doM {
+      np \<leftarrow> ll_load p; nq \<leftarrow> ll_load q;
+      b \<leftarrow> lti (node.val np) (node.val nq);
+      if to_bool b then Mreturn 1
+      else doM {
+        e \<leftarrow> eqi (node.val np) (node.val nq);
+        if to_bool e then os_less lti eqi (node.next np) (node.next nq)
+        else Mreturn 0 } })\<close>
+
+text \<open>Correctness at the owning-list level (arbitrary element assertion \<open>A\<close> over a
+  \<open>linorder\<close>). Same recursion technique as @{thm ol_eq_rule}: one \<open>subst os_less.simps\<close>
+  per case, induction hypothesis + the element rules as \<open>vcg_rules\<close>. The list-order
+  recursion lemmas are supplied locally.\<close>
+
+lemma ol_less_rule:
+  assumes LT: \<open>\<And>a c a' c'. llvm_htriple (A a c ** A a' c') (lti c c')
+    (\<lambda>r. A a c ** A a' c' ** \<upharpoonleft>bool.assn (a < a') r)\<close>
+  and EQ: \<open>\<And>a c a' c'. llvm_htriple (A a c ** A a' c') (eqi c c')
+    (\<lambda>r. A a c ** A a' c' ** \<upharpoonleft>bool.assn (a = a') r)\<close>
+  shows \<open>llvm_htriple (ol_assn A xs p ** ol_assn A ys q) (os_less lti eqi p q)
+    (\<lambda>r. ol_assn A xs p ** ol_assn A ys q ** \<upharpoonleft>bool.assn ((xs::'a::linorder list) < ys) r)\<close>
+  unfolding ol_assn_conv
+proof (induction xs arbitrary: ys p q)
+  case Nil
+  show ?case
+    supply [simp] = bool.assn_def from_bool_def list_less_Nil_left
+    apply (subst os_less.simps)
+    apply (cases ys; cases \<open>q = null\<close>; simp)
+    by vcg
+next
+  case (Cons x xs)
+  interpret llvm_prim_ctrl_setup .
+  note [vcg_rules] = Cons.IH LT EQ
+  show ?case
+    supply [simp, named_ss fri_prepare_simps] = ol_seg_cons
+    supply [simp] = bool.assn_def from_bool_def sep_conj_exists
+      list_less_Cons list_less_Nil_right
+    apply (subst os_less.simps)
+    apply (cases \<open>p = null\<close>; cases \<open>q = null\<close>; cases ys; simp)
+    by vcg
+qed
+
+lemma os_less_rule:
+  assumes P: \<open>is_pure A\<close>
+  and LT: \<open>\<And>a c a' c'. llvm_htriple (A a c ** A a' c') (lti c c')
+    (\<lambda>r. A a c ** A a' c' ** \<upharpoonleft>bool.assn (a < a') r)\<close>
+  and EQ: \<open>\<And>a c a' c'. llvm_htriple (A a c ** A a' c') (eqi c c')
+    (\<lambda>r. A a c ** A a' c' ** \<upharpoonleft>bool.assn (a = a') r)\<close>
+  shows \<open>llvm_htriple (os_assn A xs p ** os_assn A ys q) (os_less lti eqi p q)
+    (\<lambda>r. os_assn A xs p ** os_assn A ys q ** \<upharpoonleft>bool.assn ((xs::'a::linorder list) < ys) r)\<close>
+  using ol_less_rule[where A=A and lti=lti and eqi=eqi, OF LT EQ]
+  unfolding ol_assn_pure_conv[OF P] .
+
+lemma ol_less_hnr:
+  assumes LT: \<open>\<And>a c a' c'. llvm_htriple (A a c ** A a' c') (lti c c')
+    (\<lambda>r. A a c ** A a' c' ** \<upharpoonleft>bool.assn (a < a') r)\<close>
+  and EQ: \<open>\<And>a c a' c'. llvm_htriple (A a c ** A a' c') (eqi c c')
+    (\<lambda>r. A a c ** A a' c' ** \<upharpoonleft>bool.assn (a = a') r)\<close>
+  shows \<open>(uncurry (os_less lti eqi), uncurry (RETURN oo (<)))
+    \<in> (ol_assn (A :: 'a::linorder \<Rightarrow> _))\<^sup>k *\<^sub>a (ol_assn A)\<^sup>k \<rightarrow>\<^sub>a bool1_assn\<close>
+  unfolding bool1_rel_def bool.assn_is_rel[symmetric]
+  supply [vcg_rules] = ol_less_rule[OF LT EQ]
+  apply sepref_to_hoare
   apply vcg_monadify
-  apply vcg
-  sorry
+  by vcg'
 
-definition os_list_length :: \<open>'a::llvm_rep os_list \<Rightarrow> 'b::len2 word llM\<close> where [llvm_code]:
-  \<open>os_list_length p\<^sub>0 \<equiv> doM {
-    (_, i) \<leftarrow> llc_while
-      (\<lambda>(p, _). ll_cmp (p \<noteq> null))
-      (\<lambda>(p, i). doM {
-        nd \<leftarrow> ll_load p;
-        i \<leftarrow> ll_add i (signed_nat 1);
-        Mreturn (node.next nd, i)
-      }) (p\<^sub>0, signed_nat 0);
-    Mreturn i
-  }\<close>
-lemma os_list_length_rule[vcg_rules]:
-  \<open>llvm_htriple
-    (\<upharpoonleft>os_list_assn xs p)
-    (os_list_length p)
-    (\<lambda>n. \<up>(unat n = length xs) ** \<upharpoonleft>os_list_assn xs p)\<close>
-  unfolding os_list_length_def
-  apply (rewrite annotate_llc_while [where
-    I = \<open>\<lambda>(p', ii) t . EXS i. \<upharpoonleft>snat.assn i ii
-                          ** (lseg (take i xs) p p')
-                          ** (lseg (drop i xs) p' null)
-                          ** \<up>(i \<le> length xs \<and> 0 \<le> i)
-                          ** \<up>\<^sub>!(t = length xs - i)\<close>
-    and R = \<open>measure id\<close>])
-  supply [simp] = os_list_assn_def 
-  apply vcg_monadify
-  apply vcg
-  subgoal for asf i0 p' ii s i
-    apply (auto simp: STATE_def ABSTRACT_def POSTCOND_def EXTRACT_def)
-  sorry
+text \<open>Element rule for chars: \<open>ll_icmp_ult\<close> on words decides \<open>(<)\<close> on chars, because
+  \<open>char_of_word\<close> is order-preserving (unsigned word order matches char order). Proven in
+  a throwaway \<open>llvm_prim_arith_setup\<close> context, cf. @{thm char_eq_rule}.\<close>
 
-(* Now we specialize open lists to string *)
-lemma str_empty_refine[sepref_fr_rules]:
-  \<open>(uncurry0 os_empty, uncurry0 (RETURN op_list_empty)) \<in> unit_assn\<^sup>k \<rightarrow>\<^sub>a str_assn\<close>
-  unfolding os_empty_def op_list_empty_def
-  apply sepref_to_hoare
-  apply vcg
-  by (auto simp: str_assn_def ENTAILS_def entails_def os_list_assn_def hr_comp_def sep_algebra_simps)
-    
-lemma str_is_empty_refine[sepref_fr_rules]:
-  \<open>(os_is_empty, RETURN o op_list_is_empty) \<in> [\<lambda>_. True]\<^sub>a str_assn\<^sup>k \<rightarrow> bool1_assn\<close>
-  unfolding os_is_empty_def str_assn_def op_list_is_empty_def 
-  apply sepref_to_hoare
-  subgoal for x xi
-    apply (cases x; cases \<open>xi=null\<close>; simp)
-    subgoal
-      apply vcg
-      apply (simp add: sep_algebra_simps ENTAILS_def entails_def hr_comp_def os_list_assn_def)
-      by (metis bool.rel_def bool1_rel_def brI from_bool_to_bool_iff)
-    subgoal
-      apply vcg
-      by (simp add: sep_algebra_simps ENTAILS_def hr_comp_def os_list_assn_def)
-    subgoal
-      apply vcg
-      by (simp add: sep_algebra_simps ENTAILS_def hr_comp_def os_list_assn_def) 
-    subgoal
-      apply vcg
-      by (auto simp: ENTAILS_def entails_def sep_algebra_simps hr_comp_def
-        os_list_assn_def bool1_rel_def bool.rel_def in_br_conv)
-    done
-  done
+lemma char_of_word_less: \<open>char_of_word c < char_of_word c' \<longleftrightarrow> c < c'\<close>
+  using unat_of_char_mod
+  by (auto simp: char_of_word_def word_less_nat_alt PAC_Polynomials_Term.less_char_def
+      simp flip: less_char_def)
 
-lemma str_hd_refine[sepref_fr_rules]:
-  \<open>(os_hd, RETURN o op_list_hd) \<in> [\<lambda>xs. xs \<noteq> []]\<^sub>a str_assn\<^sup>k \<rightarrow> char_assn\<close>
-  unfolding str_assn_def op_list_hd_def hr_comp_def 
-  apply sepref_to_hoare
-  apply auto
-  apply vcg
-  subgoal by auto
-  subgoal
-    apply (simp add: sep_algebra_simps EXTRACT_def POSTCOND_def STATE_def list_rel_def os_list_assn_def)
-    by (metis (no_types, lifting) Sepref_Basic.pure_def char_assn_def
-    list.rel_cases list.sel(1) pred_lift_extract_simps(2) sep_conj_commuteI
-    the_pure_pure)
-  done 
+context begin
+interpretation llvm_prim_arith_setup .
 
-lemma str_tl_refine[sepref_fr_rules]:
-  \<open>(os_tl, RETURN o op_list_tl) \<in> [\<lambda>xs. xs \<noteq> []]\<^sub>a str_assn\<^sup>d \<rightarrow> str_assn\<close>
-  unfolding str_assn_def op_list_tl_def hr_comp_def
-  apply sepref_to_hoare
-  apply auto
-  apply vcg
-  subgoal by auto
-  subgoal
-    apply (simp add: sep_algebra_simps STATE_def EXTRACT_def POSTCOND_def
-            os_list_assn_def list_rel_def)
-    using list.rel_sel by blast  
-  done
-
-lemma str_prepend_refine[sepref_fr_rules]:
-  \<open>(uncurry os_prepend, uncurry (RETURN oo op_list_prepend)) \<in> char_assn\<^sup>k *\<^sub>a str_assn\<^sup>d \<rightarrow>\<^sub>a str_assn\<close>
-  unfolding str_assn_def os_prepend_def op_list_prepend_def
-  apply sepref_to_hoare
-  apply (auto simp: os_list_assn_def hr_comp_def)
-  apply vcg
-  apply (auto simp: sep_algebra_simps ENTAILS_def entails_def list_rel_def os_list_assn_def
-          char_assn_def char_rel_def in_br_conv char_of_word_def br_def)
-  by (metis (lifting) list.simps(11) lseg_Cons mem_Collect_eq old.prod.case
-    pred_lift_extract_simps(2) pure_app_eq sep_conj_aci(3))
-
-lemma str_assn_mk_free[sepref_frame_free_rules]:
-  \<open>MK_FREE str_assn os_delete\<close>
-  apply (rule MK_FREEI)
-  unfolding str_assn_def hr_comp_def 
+lemma char_lt_rule:
+  \<open>llvm_htriple (char_assn a c ** char_assn a' c') (ll_icmp_ult c c')
+    (\<lambda>r. char_assn a c ** char_assn a' c' ** \<upharpoonleft>bool.assn (a < a') r)\<close>
+  unfolding char_assn_def char_rel_def
+  supply [simp] = pure_def in_br_conv bool.assn_def char_of_word_less
   by vcg
 
-lemma str_get_refine[sepref_fr_rules]:
-  \<open>(uncurry os_list_get, uncurry (RETURN oo op_list_get)) \<in>
-  [\<lambda>(xs,i). i < length xs]\<^sub>a str_assn\<^sup>k *\<^sub>a (snat_assn' TYPE(64))\<^sup>k \<rightarrow> char_assn\<close>
-  unfolding op_list_get_def
-  apply sepref_to_hoare
-  apply (simp add: str_assn_def hr_comp_def os_list_assn_simps)
-  apply vcg
-  apply (simp add: sep_algebra_simps STATE_def EXTRACT_def POSTCOND_def snat_rel_def snat.rel_def
-    os_list_assn_def
-    snat_invar_def ll_cmp_def list_rel_def char_assn_def char_rel_def in_br_conv char_of_word_def)
-  subgoal by (metis snat_invar_def snat_eq_unat_aux2 list_all2_lengthD)
-  subgoal for bi a ai asf x sa
-    (* Residual: pick witness \<langle>x\<rangle>, then separation-logic split of the heap
-       into \<langle>os_list_assn x ai\<rangle> \<^emph> pure \<langle>char_assn (a!snat bi) (x!unat bi)\<rangle>.
-       Pattern in \<langle>str_hd_refine\<rangle> uses \<langle>list.rel_cases\<rangle> on the head; here
-       we'd need \<langle>list_all2_conv_all_nth\<rangle> at index \<langle>snat bi = unat bi\<rangle>. *)
-    sorry
-  done
+end
 
-(* NOTE: lemma as stated is not provable without a precondition like
-   \<langle>length xs < 2^(LENGTH('b) - 1)\<rangle> guaranteeing the result fits as snat.
-   After existing tactics + this auto, the residual goal is
-   \<langle>length x = snat r\<rangle> and \<langle>msb r \<Longrightarrow> False\<rangle>; the second cannot be discharged
-   without such a bound. *)
-lemma str_len_refine[sepref_fr_rules]:
-  \<open>(os_list_length, RETURN o op_list_length) \<in> str_assn\<^sup>k \<rightarrow>\<^sub>a (snat_assn' TYPE(64))\<close>
-  apply sepref_to_hoare
-  apply (simp add: str_assn_def hr_comp_def os_list_assn_simps)
-  apply vcg
-  apply (simp add: sep_algebra_simps STATE_def EXTRACT_def POSTCOND_def os_list_assn_def
-          list_rel_def char_assn_def char_rel_def in_br_conv char_of_word_def)
-  apply (auto simp: ENTAILS_def entails_def snat_rel_def snat.rel_def br_def
-          snat_invar_def list_all2_lengthD sep_algebra_simps pred_lift_extract_simps
-          snat_eq_unat)
-  sorry
+text \<open>First-order specialization for code export (recursive call folded to \<open>strl_lt\<close>).\<close>
+
+definition strl_lt :: \<open>8 word os_list \<Rightarrow> 8 word os_list \<Rightarrow> 1 word llM\<close> where
+  \<open>strl_lt \<equiv> os_less ll_icmp_ult ll_icmp_eq\<close>
+
+lemma strl_lt_simps[llvm_code]:
+  \<open>strl_lt p q = (
+    if q = null then Mreturn 0
+    else if p = null then Mreturn 1
+    else doM {
+      np \<leftarrow> ll_load p; nq \<leftarrow> ll_load q;
+      b \<leftarrow> ll_icmp_ult (node.val np) (node.val nq);
+      if to_bool b then Mreturn 1
+      else doM {
+        e \<leftarrow> ll_icmp_eq (node.val np) (node.val nq);
+        if to_bool e then strl_lt (node.next np) (node.next nq)
+        else Mreturn 0 } })\<close>
+  unfolding strl_lt_def by (rule os_less.simps)
+
+lemma strl_lt_rule[vcg_rules]:
+  \<open>llvm_htriple (strl_assn xs p ** strl_assn ys q) (strl_lt p q)
+    (\<lambda>r. strl_assn xs p ** strl_assn ys q ** \<upharpoonleft>bool.assn (xs < ys) r)\<close>
+  unfolding strl_lt_def
+  by (rule os_less_rule[where A=char_assn and lti=ll_icmp_ult and eqi=ll_icmp_eq,
+        OF char_assn_pure char_lt_rule char_eq_rule])
+
+sepref_register \<open>(<) :: char list \<Rightarrow> char list \<Rightarrow> bool\<close>
+
+lemma strl_lt_hnr[sepref_fr_rules]:
+  \<open>(uncurry strl_lt, uncurry (RETURN oo (<))) \<in> strl_assn\<^sup>k *\<^sub>a strl_assn\<^sup>k \<rightarrow>\<^sub>a bool1_assn\<close>
+  unfolding strl_lt_def
+  using ol_less_hnr[where A=char_assn and lti=ll_icmp_ult and eqi=ll_icmp_eq,
+      OF char_lt_rule char_eq_rule]
+  unfolding ol_assn_pure_conv[OF char_assn_pure] .
 
 experiment begin
+
+  definition eq_test :: \<open>str \<Rightarrow> str \<Rightarrow> bool\<close> where
+    \<open>eq_test xs ys = (xs = ys)\<close>
+
+  sepref_def eq_test_impl is \<open>uncurry (RETURN oo eq_test)\<close>
+    :: \<open>strl_assn\<^sup>k *\<^sub>a strl_assn\<^sup>k \<rightarrow>\<^sub>a bool1_assn\<close>
+    unfolding eq_test_def by sepref
+
+  definition lt_test :: \<open>str \<Rightarrow> str \<Rightarrow> bool\<close> where
+    \<open>lt_test xs ys = (xs < ys)\<close>
+
+  sepref_def lt_test_impl is \<open>uncurry (RETURN oo lt_test)\<close>
+    :: \<open>strl_assn\<^sup>k *\<^sub>a strl_assn\<^sup>k \<rightarrow>\<^sub>a bool1_assn\<close>
+    unfolding lt_test_def by sepref
 
   definition test :: \<open>str \<Rightarrow> char\<close> where
     \<open>test cs \<equiv> (if cs = [] then (char_of_word (0::(8 word))) else hd cs)\<close>
 
   sepref_def test_impl is \<open>RETURN o test\<close>
-    :: \<open>str_assn\<^sup>k \<rightarrow>\<^sub>a char_assn\<close>
-    unfolding test_def 
+    :: \<open>strl_assn\<^sup>k \<rightarrow>\<^sub>a char_assn\<close>
+    unfolding test_def
     by sepref
 
   (* export_llvm \<open>test_impl\<close> *)
@@ -225,7 +298,7 @@ experiment begin
     \<open>empty_check cs \<equiv> cs = []\<close>
 
   sepref_def empty_check_impl is \<open>RETURN o empty_check\<close>
-    :: \<open>str_assn\<^sup>k \<rightarrow>\<^sub>a bool1_assn\<close>
+    :: \<open>strl_assn\<^sup>k \<rightarrow>\<^sub>a bool1_assn\<close>
     unfolding empty_check_def
     by sepref
 
@@ -235,7 +308,7 @@ experiment begin
     \<open>cons_test cs c = c # cs\<close>
 
   sepref_def cons_test_impl is \<open>uncurry (RETURN oo cons_test)\<close>
-    :: \<open>str_assn\<^sup>d *\<^sub>a char_assn\<^sup>k \<rightarrow>\<^sub>a str_assn\<close>
+    :: \<open>strl_assn\<^sup>d *\<^sub>a char_assn\<^sup>k \<rightarrow>\<^sub>a strl_assn\<close>
     unfolding cons_test_def
     by sepref
 
@@ -243,7 +316,7 @@ experiment begin
     \<open>tail_test cs = (if cs = [] then cs else tl cs)\<close>
 
   sepref_def tail_test_impl is \<open>RETURN o tail_test\<close>
-    :: \<open>str_assn\<^sup>d \<rightarrow>\<^sub>a str_assn\<close>
+    :: \<open>strl_assn\<^sup>d \<rightarrow>\<^sub>a strl_assn\<close>
     unfolding tail_test_def
     by sepref
 
@@ -259,14 +332,21 @@ experiment begin
     | (c # cs') \<Rightarrow> c # cs'
     )\<close>
 
+  (* Pattern matching / case of does not work *)
   sepref_def dest_cons_test_impl is \<open>RETURN o dest_cons_test\<close>
-    :: \<open>str_assn\<^sup>d \<rightarrow>\<^sub>a str_assn\<close>
+    :: \<open>strl_assn\<^sup>d \<rightarrow>\<^sub>a strl_assn\<close>
     unfolding dest_cons_test_def
     apply sepref_dbg_keep
     apply sepref_dbg_trans_keep
     apply sepref_dbg_trans_step_keep
     apply sepref_dbg_side_unfold
     oops
+
+  (* But a simple workaround is to unfold list.case_eq_if *)
+  sepref_def dest_cons_test_impl' is \<open>RETURN o dest_cons_test\<close>
+    :: \<open>strl_assn\<^sup>d \<rightarrow>\<^sub>a strl_assn\<close>
+    unfolding dest_cons_test_def list.case_eq_if
+    by sepref 
 
 end
 
